src/Inline.v
@@ -212,11 +212,8 @@ Section Exts.
       match getAttribute leaf (getDefsBodies m) with
         | Some dm =>
           if noCallDm dm dm then
-            match m with
-              | Mod regs rules dms =>
-                (Mod regs (inlineDmToRules rules dm) (inlineDmToDms dms dm), true)
-              | ConcatMod m1 m2 => (m, false) (* Inlining should be done for (merge m) *)
-            end
+            (Mod (getRegInits m) (inlineDmToRules (getRules m) dm)
+                 (inlineDmToDms (getDefsBodies m) dm), true)
           else (m, false)
         | None => (m, false)
       end
